FOL/Tactics.lean
@@ -1,0 +1,35 @@
+import FOL.FOL
+import Lean
+open Lean Meta Elab Tactic
+
+partial def getAllPositions (f : Formula) : List Pos :=
+  match f with
+  | .impl f1 f2 => .root :: (getAllPositions f1).map .left ++ (getAllPositions f2).map .right
+  | .forall f1 => .root :: (getAllPositions f1).map .body
+  | _ => [.root]
+
+-- A tactic to close the goal `Γ ⊢ f` if `f ∈ Γ`.
+partial def tryMem (g : MVarId) : MetaM Unit := do
+  try
+    let _ ← g.apply (← mkConstWithFreshMVarLevels ``List.Mem.head)
+    pure ()
+  catch _ =>
+    let newGoals ← g.apply (← mkConstWithFreshMVarLevels ``List.Mem.tail)
+    if h : newGoals.length = 1 then
+      tryMem newGoals[0]
+    else
+      throwError "prove_mem failed"
+
+elab "derive_hyp" : tactic => do
+  evalTactic (← `(tactic| apply Derives.hyp))
+  let goal ← getMainGoal
+  tryMem goal
+  setGoals []
+
+-- Tactic to automate rewrite_at
+-- It tries to close the goal `Γ ⊢ f'` by finding `f ∈ Γ`, a position `p`, and a `LocalRule`
+-- such that `f` rewrites to `f'`.
+
+elab "derive_rewrite" : tactic => do
+  -- Not implemented yet, just a placeholder
+  pure ()
